Assignment 9. (a) (b) - sorried

Deduction.thy
@@ -4,8 +4,11 @@ begin
 
 (* 6. (a) *)
 
+definition \<iota> :: string where
+  "\<iota> = ''intruder''"
+
 definition intruder :: msg where
-  "intruder = Cons ''intruder''"
+  "intruder = Cons \<iota>"
 
 inductive deduce :: "msg set \<Rightarrow> msg \<Rightarrow> bool" (infix "\<turnstile>" 72) where
   Ax[intro]: "u \<in> T \<Longrightarrow> T \<turnstile> u"
@@ -170,7 +173,7 @@ inductive rer1 :: "constraint \<Rightarrow> m_subst \<Rightarrow> constraint_sys
 | Ksub: "Public_key_encrypt u (Var x) \<in> set M \<Longrightarrow> \<sigma> = Var(x := intruder) \<Longrightarrow> rer1 (M | A \<triangleright> t) \<sigma> [c_sapply \<sigma> (M | A \<triangleright> t)]"
 
 inductive rer :: "constraint_system \<Rightarrow> m_subst \<Rightarrow> constraint_system \<Rightarrow> bool" ("_/\<leadsto>[_]/_" [73,73,73]72) where
-  Context: "rer1 c \<sigma> cs \<Longrightarrow> c \<notin> set cs' \<Longrightarrow> rer (c # cs') \<sigma> (cs @ cs_sapply \<sigma> cs')"
+  Context: "rer1 c \<sigma> cs \<Longrightarrow> rer (cs' @ (c # cs'')) \<sigma> (cs @ cs_sapply \<sigma> (cs' @ cs''))"
 
 inductive rer_star :: "constraint_system \<Rightarrow> m_subst \<Rightarrow> constraint_system \<Rightarrow> bool" ("_/\<leadsto>*[_]/_" [73,73,73]72) where
   Refl: "rer_star cs Var cs"
@@ -374,7 +377,7 @@ lemma "c_fv_intruder_sub": "\<sigma> = Var(x := intruder) \<Longrightarrow> c_fv
   apply (cases c)
   using m_fv_intruder_sub by fastforce+
 
-lemma "rer1_fv_sub_cs": "rer1 c \<sigma> cs \<Longrightarrow> cs_fv cs \<subseteq> cs_fv (c # cs')"
+lemma "rer1_fv_sub_cs_aux": "rer1 c \<sigma> cs \<Longrightarrow> cs_fv cs \<subseteq> cs_fv (c # cs'')"
   unfolding cs_fv_def cs_sapply_def
   using c_fv_intruder_sub
   apply -
@@ -385,7 +388,11 @@ proof (induction rule: rer1.induct)
     by (metis Union_iff image_iff list.distinct(1) list.set_cases list.set_intros(1) set_ConsD subsetCE)
 qed auto
 
-lemma "rer1_fv_sub_cs'": "rer1 c \<sigma> cs \<Longrightarrow> cs_fv (cs_sapply \<sigma> cs') \<subseteq> cs_fv (c # cs')"
+lemma "rer1_fv_sub_cs": "rer1 c \<sigma> cs \<Longrightarrow> cs_fv cs \<subseteq> cs_fv (cs' @ (c # cs''))"
+  using rer1_fv_sub_cs_aux
+  using cs_fv_def by fastforce
+
+lemma "rer1_fv_sub_cs'": "rer1 c \<sigma> cs \<Longrightarrow> cs_fv (cs_sapply \<sigma> (cs' @ cs'')) \<subseteq> cs_fv (cs' @ (c # cs''))"
   unfolding cs_fv_def cs_sapply_def
   using cs_sapply_id c_sapply_id
   apply -
@@ -399,7 +406,7 @@ proof (induction rule: rer1.induct)
   then have "m_svran \<sigma> \<subseteq> c_fv (M | A \<triangleright> t)"
     using $
     by auto
-  then have "cs_fv (cs_sapply \<sigma> cs') \<subseteq> cs_fv cs' \<union> c_fv (M | A \<triangleright> t)"
+  then have "cs_fv (cs_sapply \<sigma> (cs' @ cs'')) \<subseteq> cs_fv (cs' @ cs'') \<union> c_fv (M | A \<triangleright> t)"
     using cs_fv_sapply_sdom_svran
     by blast
   then show ?case
@@ -410,16 +417,15 @@ next
   show ?case
     apply (rule subsetI)
     apply simp
-    apply (rule disjI2)+
     using Ksub.hyps(2) c_fv_intruder_sub by blast
 qed auto
 
-lemma "rer1_fv_sub": "rer1 c \<sigma> cs \<Longrightarrow> cs_fv (cs @ cs_sapply \<sigma> cs') \<subseteq> cs_fv (c # cs')"
+lemma "rer1_fv_sub": "rer1 c \<sigma> cs \<Longrightarrow> cs_fv (cs @ cs_sapply \<sigma> (cs' @ cs'')) \<subseteq> cs_fv (cs' @ (c # cs''))"
   using rer1_fv_sub_cs rer1_fv_sub_cs'
   unfolding cs_fv_def
   by auto
 
-lemma "rer1_fv_neq": "rer1 c \<sigma> cs \<Longrightarrow> \<sigma> \<noteq> Var \<Longrightarrow> cs_fv (cs @ cs_sapply \<sigma> cs') \<noteq> cs_fv (c # cs')"
+lemma "rer1_fv_neq": "rer1 c \<sigma> cs \<Longrightarrow> \<sigma> \<noteq> Var \<Longrightarrow> cs_fv (cs @ cs_sapply \<sigma> (cs' @ cs'')) \<noteq> cs_fv (cs' @ (c # cs''))"
 proof (induction rule: rer1.induct)
   case (Unif t M A \<sigma>)
   then obtain "u" "x" where $: "u \<in> set M \<union> set A" and "m_un": "m_unify [(t, u)] = Some \<sigma>" and "x_m_sdom": "x \<in> m_sdom \<sigma>"
@@ -429,17 +435,17 @@ proof (induction rule: rer1.induct)
   then have "m_sdom \<sigma> \<subseteq> c_fv (M | A \<triangleright> t)"
     using $
     by auto
-  then have "x_cs_fv": "x \<in> cs_fv ((M | A \<triangleright> t) # cs')"
+  then have "x_cs_fv": "x \<in> cs_fv (cs' @ (M | A \<triangleright> t) # cs'')"
     unfolding cs_fv_def
     using "x_m_sdom"
     by auto
-  have "cs_fv (cs_sapply \<sigma> cs') \<subseteq>  cs_fv cs' - m_sdom \<sigma> \<union> m_svran \<sigma>"
+  have "cs_fv (cs_sapply \<sigma> (cs' @ cs'')) \<subseteq>  cs_fv (cs' @ cs'') - m_sdom \<sigma> \<union> m_svran \<sigma>"
     using cs_fv_sapply_sdom_svran
     by blast
   have "m_sdom \<sigma> \<inter> m_svran \<sigma> = {}"
     using m_lemma_3 m_un
     by blast
-  then have "x \<notin> cs_fv ([] @ (cs_sapply \<sigma> cs'))"
+  then have "x \<notin> cs_fv ([] @ (cs_sapply \<sigma> (cs' @ cs'')))"
     using cs_fv_sapply_sdom_svran x_m_sdom
     by fastforce
   then show ?case
@@ -448,14 +454,14 @@ proof (induction rule: rer1.induct)
     by auto
 next
   case (Ksub u x M \<sigma> A t)
-  then have "x_in_cs_fv": "x \<in> cs_fv (M | A \<triangleright> t # cs')"
+  then have "x_in_cs_fv": "x \<in> cs_fv (cs' @ (M | A \<triangleright> t # cs''))"
     unfolding cs_fv_def
     by fastforce
   have "x \<in> m_sdom \<sigma> - m_svran \<sigma>"
     using Ksub.hyps
     unfolding intruder_def
     by simp
-  then have "x \<notin> cs_fv (cs_sapply \<sigma> ((M | A \<triangleright> t) # cs'))"
+  then have "x \<notin> cs_fv (cs_sapply \<sigma> (cs' @ (M | A \<triangleright> t) # cs''))"
     using Ksub.hyps cs_fv_sapply_sdom_svran
     unfolding cs_fv_def cs_sapply_def
     by blast
